isabelle/Auction/ListUtils.thy
@@ -21,7 +21,7 @@ theory ListUtils
 imports Main
 begin
 
-(* norepetitions is the same as List.distinct *)
+(* MC's old norepetitions is the same as List.distinct *)
 
 lemma distinct_imp_card_eq_length: "distinct l \<longleftrightarrow> card (set l) = length l"
   by (metis card_distinct length_remdups_card_conv remdups_id_iff_distinct)
@@ -29,13 +29,15 @@ lemma distinct_imp_card_eq_length: "distinct l \<longleftrightarrow> card (set l
 lemma "distinct l \<longleftrightarrow> (card (set l) \<ge> length l)" 
   using distinct_imp_card_eq_length by (metis card_length le_antisym)
 
-(* noreptl existed in the library as List.distinct_tl *)
+(* MC's old noreptl existed in the library as List.distinct_tl *)
 
 lemma finite_imp_length_sort_eq_card: fixes x assumes "finite x"
   shows "length (sorted_list_of_set x) = card x"
   using assms
   by (metis distinct_imp_card_eq_length sorted_list_of_set)
 
-(* setlistid and norepset exist in the library as List.sorted_list_of_set *)
+(* MC's old setlistid and norepset exist in the library as List.sorted_list_of_set *)
+
+lemma remove_list_to_set: "set (x # removeAll y l) = insert x (set l - {y})" by simp
 
 end
